theories/Factor_Self_Contained_Terms.thy
@@ -257,11 +257,7 @@ lemma data_collection_presents_map:
 lemma data_collection_presents_function:
   "data_collection_presents (\<lambda>a u. u=f a) A t \<longleftrightarrow>
     (\<exists>xs. distinct xs \<and> set xs=A \<and> t=data_list_term (map f xs))"
-proof -
-  have related: "list_all2 (\<lambda>a u. u=f a) xs ts \<longleftrightarrow> ts=map f xs" for xs ts
-    by (induction xs arbitrary: ts) (auto simp: list_all2_Cons1)
-  show ?thesis by (simp add: data_collection_presents_def related)
-qed
+  by (simp add: data_collection_presents_def list_all2_function)
 
 lemma data_collection_presents_total:
   assumes fin: "finite A" and each: "\<forall>a\<in>A. \<exists>t. read a t"
